src/Unfolder.v
@@ -20,6 +20,48 @@ Fixpoint allb A (P : A -> bool) (ls : list A) : bool :=
     | x :: ls' => P x && allb P ls'
   end.
 
+Lemma nth_error_None_length : forall (T : Type) (ls : list T) (n : nat),
+  nth_error ls n = None -> length ls <= n.
+Proof.
+  induction ls; destruct n; simpl; intros; think; try omega. inversion H.
+  eapply IHls in H. omega.
+Qed.
+
+Lemma applyD_impl_Forall : forall types F F' P Dom args R D v,
+  applyD (types := types) F Dom args R D = Some v ->
+  Forall P args ->
+  (forall x y v, P x -> F x y = Some v -> F' x y = Some v) ->
+  applyD F' Dom args R D = Some v.
+Proof.
+  induction Dom; destruct args; simpl; intros; think; auto. inversion H0; subst; intros.
+  erewrite H1; eauto.
+Qed.
+
+Lemma applyD_impl : forall types F F' Dom args R D,
+  (forall x y, F x y = F' x y) ->
+  applyD (types := types) F Dom args R D = applyD F' Dom args R D.
+Proof.
+  induction Dom; destruct args; simpl; intros; think; auto.
+  destruct (F' e a); auto.
+Qed.
+
+Lemma applyD_map : forall types F F' Dom args R D,
+  applyD (types := types) F Dom (map F' args) R D = applyD (fun x y => F (F' x) y) Dom args R D.
+Proof.
+  induction Dom; destruct args; simpl; intros; think; auto.
+  destruct (F (F' e) a); auto.
+Qed.
+
+Lemma map_nth_error_full : forall T U (F : T -> U) ls n,
+  nth_error (map F ls) n = match nth_error ls n with
+                             | None => None
+                             | Some v => Some (F v)
+                           end.
+Proof.
+  induction ls; destruct n; simpl; intros; think; auto.
+Qed.
+
+
 Module Make (SH : SepHeap) (U : SynUnifier).
   Module Import SE := SH.SE.
   Import SH.
@@ -41,67 +83,83 @@ Module Make (SH : SepHeap) (U : SynUnifier).
 
     (** * Some substitution functions *)
 
-    (* [firstVar]: Add this to all indices of variables appearing within [e].
-     * [firstFree] tells us which is the first regular variable to be treated as a unification variable. *)
-    Fixpoint substExpr (firstVar firstFree : nat) (s : U.Subst types) (e : expr types) : expr types :=
-      match e with
-        | Expr.Const _ _ => e
-        | Var x => if NPeano.ltb x firstFree
-          then Var (x + firstVar)
-          else match U.Subst_lookup (x - firstFree) s with
-                 | None => e
-                 | Some e' => e'
-               end
-        | UVar _ => e
-        | Expr.Func f es => Expr.Func f (map (substExpr firstVar firstFree s) es)
-        | Equal t e1 e2 => Equal t (substExpr firstVar firstFree s e1) (substExpr firstVar firstFree s e2)
-        | Not e1 => Not (substExpr firstVar firstFree s e1)
-      end.
+    Section openForUnification.
+      Variable U : nat. (** **)
 
-    Definition substSheap (firstVar firstFree : nat) (s : U.Subst types) (sh : SHeap types pcType stateType)
-      : SHeap types pcType stateType :=
-      {| impures := MM.mmap_map (map (substExpr firstVar firstFree s)) (impures sh)
-       ; pures := map (substExpr firstVar firstFree s) (pures sh)
+      Definition ERROR : expr types.
+      refine (Var 0).
+      Qed.
+      
+      Fixpoint openForUnification (e : expr types) : expr types :=
+        match e with
+          | Expr.Const _ _ => e
+          | Var v => UVar (U + v)
+          | UVar _ => e (** contradiction **)
+          | Expr.Func f es => Expr.Func f (List.map openForUnification es)
+          | Equal t l r => Equal t (openForUnification l) (openForUnification r)
+          | Not e => Not (openForUnification e)
+        end.
+
+    End openForUnification.
+
+    Section instantiate.
+      Variable doQuant : nat -> expr types.
+      Variable U : nat.
+      Variable G' : nat.
+      Variable sub : U.Subst types.
+      
+      Fixpoint liftInstantiate (e : expr types) : expr types :=
+        match e with
+          | Expr.Const _ _ => e
+          | Var v => 
+            if NPeano.ltb v G' then doQuant v (* Var (v + G) *)
+            else let idx := U + v - G' in 
+                 match U.Subst_lookup idx sub with
+                   | None => UVar idx (** contradiction **)
+                   | Some e => e
+                 end
+          | UVar v => match U.Subst_lookup v sub with (** contradiction **)
+                        | None => UVar v
+                        | Some e => e
+                      end
+          | Expr.Func f es => Expr.Func f (List.map liftInstantiate es)
+          | Equal t l r => Equal t (liftInstantiate l) (liftInstantiate r)
+          | Not e => Not (liftInstantiate e)
+        end.
+
+    End instantiate.
+
+    Definition quantFwd (over : nat) (v : nat) : expr types :=  Var (v + over).
+    Definition quantBwd (over : nat) (v : nat) : expr types :=  UVar (v + over).
+
+    Class QuantifierSpec U G (quant : nat -> expr types) (BuildUVars BuildVars : env types -> env types -> env types) : Prop :=
+    { Weakenable : forall funcs F e t v, 
+      exprD funcs U G e t = Some v ->
+      exprD funcs (BuildUVars U F) (BuildVars G F) e t = Some v
+    ; PreservesVar : 
+      forall funcs F v t,
+      is_well_typed (typeof_funcs funcs) nil (typeof_env F) (Var (types := types) v) t = true ->
+      exprD funcs nil F (Var v) t = exprD funcs (BuildUVars U F) (BuildVars G F) (quant v) t
+    }.
+    Instance QuantifierSpec_Fwd U G : QuantifierSpec U G (quantFwd (length G)) (fun x _ => x) (fun x y => x ++ y).
+    constructor.
+    { intros. rewrite <- app_nil_r with (l := U). eapply exprD_weaken; auto. }
+    { intros. simpl; unfold lookupAs; simpl.
+      rewrite nth_error_app_R. cutrewrite (v + length G - length G = v); [ | omega ]. reflexivity. omega. }
+    Qed.
+
+    Instance QuantifierSpec_Bwd U G : QuantifierSpec U G (quantBwd (length U)) (fun x y => x ++ y) (fun x _ => x).
+    constructor.
+    { intros. rewrite <- app_nil_r with (l := G). eapply exprD_weaken; auto. }
+    { intros. simpl; unfold lookupAs; simpl.
+      rewrite nth_error_app_R. cutrewrite (v + length U - length U = v); [ | omega ]. reflexivity. omega. }
+    Qed.
+
+    Definition applySHeap (F : expr types -> expr types) (sh : SHeap types pcType stateType) : SHeap types pcType stateType :=
+      {| impures := MM.mmap_map (map F) (impures sh)
+       ; pures := map F (pures sh)
        ; other := other sh
        |}.
-
-    Fixpoint substExprBw (offset firstFree : nat) (s : U.Subst types) (e : expr types) : expr types :=
-      match e with
-        | Expr.Const _ _ => e
-        | Var x => if NPeano.ltb x firstFree
-          then e
-          else match U.Subst_lookup (x - firstFree + offset) s with
-                 | None => e
-                 | Some e' => e'
-               end
-        | UVar _ => e
-        | Expr.Func f es => Expr.Func f (map (substExprBw offset firstFree s) es)
-        | Equal t e1 e2 => Equal t (substExprBw offset firstFree s e1) (substExprBw offset firstFree s e2)
-        | Not e1 => Not (substExprBw offset firstFree s e1)
-      end.
-
-    Fixpoint substExprBw' (offset firstFree : nat) (s : U.Subst types) (e : expr types) : expr types :=
-      match e with
-        | Expr.Const _ _ => e
-        | Var x => if NPeano.ltb x firstFree
-          then UVar (x + offset)
-          else match U.Subst_lookup (x - firstFree + offset) s with
-                 | None => e
-                 | Some e' => e'
-               end
-        | UVar _ => e
-        | Expr.Func f es => Expr.Func f (map (substExprBw' offset firstFree s) es)
-        | Equal t e1 e2 => Equal t (substExprBw' offset firstFree s e1) (substExprBw' offset firstFree s e2)
-        | Not e1 => Not (substExprBw' offset firstFree s e1)
-      end.
-
-    Definition substSheapBw (offset firstFree : nat) (s : U.Subst types) (sh : SHeap types pcType stateType) 
-      : SHeap types pcType stateType :=
-      {| impures := MM.mmap_map (map (substExprBw' offset firstFree s)) (impures sh)
-       ; pures := map (substExprBw' offset firstFree s) (pures sh)
-       ; other := other sh
-       |}.
-
 
     (** The type of one unfolding lemma *)
     Record lemma := {
@@ -143,7 +201,7 @@ Module Make (SH : SepHeap) (U : SynUnifier).
       end.
 
     Definition lemmaD (meta_base var_base : env types) (lem : lemma) : Prop :=
-      WellTyped_lemma (typeof_funcs funcs) (Predicates_typeof preds) lem = true /\
+      WellTyped_lemma (typeof_funcs funcs) (typeof_preds preds) lem = true /\
       forallEachR (Foralls lem) (fun env =>
         implyEach (Hyps lem) meta_base (var_base ++ env)
         (forall specs, himp funcs preds meta_base (var_base ++ env) specs (Lhs lem) (Rhs lem))).
@@ -163,9 +221,9 @@ Module Make (SH : SepHeap) (U : SynUnifier).
     }.
 
     Definition default_hintsPayload : hintsPayload := 
-    {| Forward := nil
-     ; Backward := nil
-     |}.
+      {| Forward := nil
+       ; Backward := nil
+       |}.
 
     Definition composite_hintsPayload (l r : hintsPayload) : hintsPayload :=
       {| Forward := Forward l ++ Forward r
@@ -279,22 +337,22 @@ Module Make (SH : SepHeap) (U : SynUnifier).
           | nil => true
           | _ :: ts => if U.Subst_lookup from sub then checkAllInstantiated (S from) ts sub else false
         end.
-
-
+      
       (** Determine if a lemma is applicable.
        ** - [firstUVar] an index larger than the largest unification variable
        ** - [lem] is the lemma to apply
        ** - [args] is the outside
        ** - [key] is the patterns (closed by [Foralls lem]) that need to unify with [args])
        **)
-      Definition applicable (asrt : bool) (firstUvar : nat) (lem : lemma) (args key : exprs types) : option (U.Subst types) :=
+      Definition applicable quant (firstUvar : nat) (lem : lemma) (args key : exprs types) 
+        : option (U.Subst types) :=
         let numForalls := length (Foralls lem) in
-        match fold_left_2_opt (U.exprUnify unify_bound) args (map (exprSubstU 0 numForalls firstUvar) key) (U.Subst_empty _) with
+        match fold_left_2_opt (U.exprUnify unify_bound) args (map (openForUnification firstUvar) key) (U.Subst_empty _) with
           | None => None
           | Some subst =>
-            (* Now we must make sure all of the lemma's pure obligations are provable. *)
-            if allb (Prove prover facts) (map (substExpr firstUvar O subst) (Hyps lem))
-            then if true (* (if asrt then EqNat.beq_nat (U.Subst_size subst) numForalls else true) && checkAllInstantiated 0 (Foralls lem) subst *)
+            if EqNat.beq_nat (U.Subst_size subst) numForalls && checkAllInstantiated firstUvar (Foralls lem) subst
+            then (* Now we must make sure all of the lemma's pure obligations are provable. *)
+                 if allb (Prove prover facts) (map (liftInstantiate quant firstUvar 0 subst) (Hyps lem))
                  then Some subst
                  else None
             else None
@@ -316,7 +374,7 @@ Module Make (SH : SepHeap) (U : SynUnifier).
                   findWithRest (fun args argss =>
                     (* We must tweak the arguments by substituting unification variables for 
                      * [forall]-quantified variables from the lemma statement. *)
-                    match applicable false firstUvar h args args' with
+                    match applicable (quantFwd firstVar) firstUvar h args args' with
                       | None => None 
                       | Some subs =>
 (*
@@ -340,7 +398,7 @@ Module Make (SH : SepHeap) (U : SynUnifier).
                           let (exs, sh') := hash (Rhs h) in
 
                           (* Apply the substitution that unification gave us. *)
-                          let sh' := substSheap firstVar (length exs) subs sh' in
+                          let sh' := applySHeap (liftInstantiate (quantFwd firstVar) firstUvar (length exs) subs) sh' in
 
                           (* The final result is obtained by joining the hint RHS with the original symbolic heap. *)
                           Some {| Vars := Vars s ++ rev exs
@@ -358,8 +416,9 @@ Module Make (SH : SepHeap) (U : SynUnifier).
           end) hs.
      
       Definition unfoldBackward (s : unfoldingState) : option unfoldingState :=
-        let imps := SH.impures (Heap s) in
-        let firstUvar := length (UVars s) in
+        let imps       := SH.impures (Heap s) in
+        let firstUvar  := length (UVars s) in
+        let firstVar   := length (Vars s) in
         find (fun h =>
           match Rhs h with
             | Func f args' =>
@@ -367,10 +426,10 @@ Module Make (SH : SepHeap) (U : SynUnifier).
                 | None => None
                 | Some argss => 
                   findWithRest (fun args argss =>
-(*                    match applicable false firstUvar h args args' with
+                    match applicable (quantBwd firstUvar) firstUvar h args args' with
                       | None => None
                       | Some subs =>
-*)
+(*
                     let args' := map (exprSubstU O (length (Foralls h)) firstUvar) args' in
 
                     (* Unify the respective function arguments. *)
@@ -379,6 +438,7 @@ Module Make (SH : SepHeap) (U : SynUnifier).
                       | Some subs =>
                         (* Now we must make sure all of the lemma's pure obligations are provable. *)
                         if allb (Prove prover facts) (map (substExprBw firstUvar O subs) (Hyps h)) then
+*)
                           (* Remove the current call from the state, as we are about to replace it with a 
                            * simplified set of pieces. *)
                           let impures' := FM.add f argss (impures (Heap s)) in
@@ -391,15 +451,17 @@ Module Make (SH : SepHeap) (U : SynUnifier).
 
                           (* Newly introduced variables must be replaced with unification variables, and 
                            * universally quantified variables must be substituted for. *)
-                          let sh' := substSheapBw firstUvar (length exs) subs sh' in
+                          let sh' := applySHeap (liftInstantiate (quantBwd firstUvar) firstUvar (length exs) subs) sh' in
 
                           (* The final result is obtained by joining the hint LHS with the original symbolic heap. *)
                           Some {| Vars := Vars s
                                 ; UVars := UVars s ++ rev exs
                                 ; Heap := star_SHeap sh sh'
                                 |}
+(*
                         else
                           None
+*)
                     end
                   ) argss
               end
@@ -464,35 +526,141 @@ Module Make (SH : SepHeap) (U : SynUnifier).
         f_equal. eauto.
       Qed.
 
-
-      Theorem unify_args_forallEachR : forall tfuncs tU tG U G l r D (S : U.Subst types) S' P env cur TS,
-        U.Subst_WellTyped tfuncs tU tG S ->
-        all2 (@is_well_typed _ tfuncs tU tG) l D = true ->
-        all2 (@is_well_typed _ tfuncs tU tG) r D = true ->
-        fold_left_2_opt (U.exprUnify unify_bound) l r S = Some S' ->
-        Subst_to_env U G S' TS cur = Some env ->
-        forallEachR TS P ->
-        P env.
+      Lemma Subst_to_env_nth_error_lookup : forall F U G sub x v CUR,
+        Subst_to_env U G sub (typeof_env F) CUR = Some F ->
+        nth_error F x = Some v ->
+        exists e, U.Subst_lookup (CUR + x) sub = Some e /\
+          exprD funcs U G e (projT1 v) = Some (projT2 v).
       Proof.
-        clear.
-        induction l; destruct TS; try congruence; simpl in *; intros;
+        induction F; simpl; intros; think.
+        { destruct x; simpl in *; unfold error in *; congruence. }
+        { destruct a; simpl in *. think. apply inj_pair2 in H5. subst.
+          destruct x; simpl in *. 
+          { inversion H0; clear H0; subst. rewrite Plus.plus_0_r. eexists; intuition eauto. }
+          { rewrite Plus.plus_comm. simpl. rewrite Plus.plus_comm. eapply IHF in H1. simpl in H1. eapply H1. auto. } }
+      Qed.
+      Lemma Subst_to_env_typeof_env : forall U G sub ts CUR F,
+        Subst_to_env U G sub ts CUR = Some F ->
+        ts = typeof_env F.
+      Proof.
+        induction ts; simpl; intros.
+        { think. reflexivity. }
+        { consider (Subst_to_env U G sub ts (S CUR)). intros. eapply IHts in H. think. simpl. auto.
+          intros; think. }
+      Qed.
+
+      Lemma nth_error_typeof_funcs : forall f t s,
+        nth_error (typeof_funcs funcs) f = Some t ->
+        nth_error funcs f = Some s ->
+        TRange t = Range s /\ TDomain t = Domain s.
+      Proof.
+        unfold typeof_funcs. intros. erewrite map_nth_error in H by eauto. think. unfold typeof_sig; intuition.
+      Qed.
+
+      Lemma typeof_env_length : forall types g, 
+        length (typeof_env (types := types) g) = length g.
+      Proof.
+        intros. apply map_length.
+      Qed.
+
+      Theorem openForUnification_spec : forall F U G e t ,
+        is_well_typed (typeof_funcs funcs) nil (typeof_env F) e t = true ->
+        exprD funcs nil F e t = exprD funcs (U ++ F) G (openForUnification (length U) e) t.
+      Proof.
+        induction e; simpl; unfold lookupAs; intros; think;
           repeat match goal with
-                   | [ H : Some _ = Some _ |- _ ] => inversion H; clear H; subst
-                   | [ H : context [ match ?X with _ => _ end ] |- _ ] =>
-                     revert H ; case_eq X ; intros; try congruence
-                   | [ |- _ ] => progress ( simpl in * )
-                   | [ |- _ ] => progress subst
-                   | [ H : U.exprUnify _ _ _ _ = Some _ |- _ ] => 
-                     generalize H ; generalize H; 
-                     apply U.exprUnify_Extends in H ;
-                     let H := fresh "H" in
-                     intro H ;
-                     apply U.exprUnify_sound in H
-                 end; try solve [ intuition ].
-        eapply forallEachR_sem in H4. eapply H4.
-        eauto using Subst_to_env_env.        
-        
-        intro. eapply IHl in H4. eapply H4. 4: eauto. eauto using U.exprUnify_WellTyped. eauto. eauto. eauto.
+                   | [ H : nth_error _ _ = Some _ |- _ ] =>  
+                     eapply WellTyped_env_nth_error_Some in H; [ | solve [ eauto using typeof_env_WellTyped_env ] ] ; destruct H
+                   | [ |- _ ] => rewrite nth_error_app_R by omega
+                   | [ |- _ ] => rewrite nth_error_app_L by omega
+                   | [ H : nth_error ?L ?n = _ |- context [ nth_error ?L ?n' ] ] =>
+                     cutrewrite (n' = n); [ | omega ]
+                   | [ H : nth_error nil ?X = Some _ |- _ ] =>
+                     clear - H ; abstract (exfalso ; destruct X ; simpl in *; unfold error in *; congruence)
+                   | [ |- match ?X with _ => _ end = match ?X with _ => _ end ] =>
+                     consider X; intros; try reflexivity
+                 end; think; auto.
+        eapply nth_error_typeof_funcs in H2; eauto. intuition. think.
+        { rewrite applyD_map.
+          revert H1. destruct s; simpl in *. clear H5. generalize dependent Domain. clear - H.
+          induction H; destruct Domain; intros; simpl in *; think; auto.
+          consider (exprD funcs (U ++ F) G (openForUnification (length U) x) t); intros; auto. }
+      Qed.
+
+      Theorem openForUnification_typed : forall F U G e t ,
+        is_well_typed (typeof_funcs funcs) nil F e t = true ->
+        is_well_typed (typeof_funcs funcs) (U ++ F) G (openForUnification (length U) e) t = true.
+      Proof.
+        induction e; simpl; unfold lookupAs; intros; think;
+          repeat match goal with
+                   | [ H : nth_error _ _ = Some _ |- _ ] =>  
+                     eapply WellTyped_env_nth_error_Some in H; [ | solve [ eauto using typeof_env_WellTyped_env ] ] ; destruct H
+                   | [ |- _ ] => rewrite nth_error_app_R by omega
+                   | [ |- _ ] => rewrite nth_error_app_L by omega
+                   | [ H : nth_error ?L ?n = _ |- context [ nth_error ?L ?n' ] ] =>
+                     cutrewrite (n' = n); [ | omega ]
+                   | [ H : nth_error nil ?X = Some _ |- _ ] =>
+                     clear - H ; abstract (exfalso ; destruct X ; simpl in *; unfold error in *; congruence)
+                   | [ |- match ?X with _ => _ end = match ?X with _ => _ end ] =>
+                     consider X; intros; try reflexivity
+                 end; think; auto.
+        { rewrite EquivDec_refl_left. reflexivity. }
+        { destruct t0; simpl in *. clear H0. generalize dependent TDomain. induction H; destruct TDomain; simpl in *; auto.
+          intros; think; auto. }
+      Qed.
+
+      Theorem liftInstantiate_spec : forall U G quant (BuildUVars BuildVars : env types -> env types -> env types),
+        QuantifierSpec U G quant BuildUVars BuildVars ->
+        forall G' F e t sub ts,
+          is_well_typed (typeof_funcs funcs) nil (typeof_env G' ++ typeof_env F) e t = true ->
+          Subst_to_env U G sub ts (length U) = Some F ->
+          exprD funcs nil (G' ++ F) e t =
+          exprD funcs (BuildUVars U G') (BuildVars G G') (liftInstantiate quant (length U) (length G') sub e) t.
+      Proof.
+        induction e; repeat progress (simpl in *; unfold lookupAs in *; intros; 
+          repeat match goal with
+                   | [ H : nth_error _ _ = Some _ |- _ ] =>  
+                     eapply WellTyped_env_nth_error_Some in H; [ | solve [ eauto using typeof_env_WellTyped_env ] ] ; destruct H
+                   | [ |- _ ] => rewrite nth_error_app_R by omega
+                   | [ |- _ ] => rewrite nth_error_app_L by omega
+                   | [ |- _ ] => rewrite nth_error_app_R in * by omega
+                   | [ |- _ ] => rewrite nth_error_app_L in * by omega
+                   | [ H : nth_error ?L ?n = _ |- context [ nth_error ?L ?n' ] ] =>
+                     cutrewrite (n' = n); [ | omega ]
+                   | [ H : nth_error nil ?X = Some _ |- _ ] =>
+                     clear - H ; abstract (exfalso ; destruct X ; simpl in *; unfold error in *; congruence)
+                   | [ |- match ?X with _ => _ end = match ?X with _ => _ end ] =>
+                     consider X; intros; try reflexivity
+                   | [ |- context [ NPeano.ltb ?X ?Y ] ] => consider (NPeano.ltb X Y); intros
+                 end; think); auto.
+        { eapply H. rewrite nth_error_app_L in H0. simpl in *. unfold typeof_env in *. 
+          repeat rewrite map_nth_error_full in *. consider (nth_error G' x). intros; think.
+          rewrite EquivDec_refl_left. auto. congruence. rewrite typeof_env_length. auto. }
+        { rewrite nth_error_app_R in H0. 2: rewrite typeof_env_length; auto.
+          rewrite typeof_env_length in *. unfold typeof_env in *. rewrite map_nth_error_full in *.
+          generalize (Subst_to_env_typeof_env _ _ _ _ _ H1); intros; subst.
+          consider (nth_error F (x - length G')); intros; try congruence.
+          eapply Subst_to_env_nth_error_lookup in H1; eauto. inversion H3; clear H3; subst. destruct H1. intuition.
+          cutrewrite (length U + (x - length G') = length U + x - length G') in H3; [ | omega ].
+          rewrite H3. rewrite EquivDec_refl_left. symmetry. eapply Weakenable. eauto. }
+        { unfold typeof_funcs in H1; rewrite map_nth_error_full in H1. rewrite H3 in H1. inversion H1; clear H1; subst.
+          unfold typeof_sig in *. simpl in *. destruct s. revert H5 H2. clear - H0. generalize dependent Domain.
+          induction H0; destruct Domain; simpl in *; intros; think; auto.
+          erewrite <- H; eauto. destruct (exprD funcs nil (G' ++ F) x t); auto. }
+      Qed.
+
+      Theorem liftInstantiate_typed : forall U G quant (BuildUVars BuildVars : env types -> env types -> env types),
+        QuantifierSpec U G quant BuildUVars BuildVars ->
+        forall G' F e t sub ts,
+          is_well_typed (typeof_funcs funcs) nil (typeof_env G' ++ typeof_env F) e t = true ->
+          Subst_to_env U G sub ts (length U) = Some F ->
+          is_well_typed (typeof_funcs funcs) nil (typeof_env (G' ++ F)) e t = true ->
+          is_well_typed (typeof_funcs funcs) (typeof_env (BuildUVars U G')) (typeof_env (BuildVars G G')) 
+          (liftInstantiate quant (length U) (length G') sub e) t = true.
+      Proof.
+        intros. eapply is_well_typed_correct in H2; eauto using typeof_env_WellTyped_env, typeof_funcs_WellTyped_funcs.
+        2: instantiate (1 := nil); reflexivity. destruct H2. erewrite liftInstantiate_spec in H2 by eassumption.
+        eapply is_well_typed_correct_only in H2; eauto using typeof_env_WellTyped_env, typeof_funcs_WellTyped_funcs.
       Qed.
 
       Lemma is_well_typed_weaken : forall tf tU tG e t,
@@ -514,7 +682,6 @@ Module Make (SH : SepHeap) (U : SynUnifier).
         consider (is_well_typed tf tU tG x t); intros. erewrite H by eauto. eauto.
       Qed.
 
-
       Lemma all2_is_well_typed_weaken : forall tf tU tG es ts,
         all2 (is_well_typed (types := types) tf tU tG) es ts = true ->
         forall u g,
@@ -522,46 +689,7 @@ Module Make (SH : SepHeap) (U : SynUnifier).
       Proof.
         clear. intros. eapply all2_impl; eauto using is_well_typed_weaken.
       Qed.
-
-      Lemma exprSubstU_WellTyped : forall tf tU tG ext (a : expr types) t,
-        is_well_typed tf tU (tG ++ ext) a t = true ->
-        is_well_typed tf (tU ++ ext) tG (exprSubstU (length tG) (length tG + length ext) (length tU) a) t = true.
-      Proof.
-(*
-        clear. induction a; simpl; intros; 
-        repeat match goal with
-                 | [ H : match ?X with tvProp => _ | tvType _ => _ end = _ |- _ ] =>
-                   destruct X; try congruence
-                 | [ H : (_ && _) = true |- _ ] => apply andb_true_iff in H; destruct H
-                 | [ H : _ |- _ ] => rewrite H by auto
-                 | [ |- context [ if NPeano.ltb ?A ?B then _ else _ ] ] =>
-                   consider (NPeano.ltb A B); intros
-                 | [ |- _ ] => 
-                   rewrite nth_error_app_L by omega
-                 | [ |- _ ] => rewrite nth_error_app_R by omega
-                 | [ H : _ |- _ ] => 
-                   rewrite nth_error_app_R in H by omega 
-                 | [ H : _ |- _ ] => 
-                   rewrite nth_error_app_L in H by omega 
-                 | [ |- _ ] => progress ( simpl in * )
-                 | [ H : match nth_error _ ?X with _ => _ end = _ |- match nth_error _ ?Y with _ => _ end = _ ] => 
-                   cutrewrite (Y = X); [ auto | omega ] 
-               end; auto.
-        { exfalso. consider (nth_error ext (x - length tG)); intros. apply nth_error_Some_length in H. omega. }
-        { consider (nth_error tU x); intros. erewrite nth_error_weaken by eauto. auto. }
-        { consider (nth_error tf f); intros. consider (equiv_dec t (TRange t0)); intros.
-          unfold equiv in *; simpl in *; subst. clear H0. generalize dependent (TDomain t0). 
-          induction H; intros; simpl in *; think; auto; intros; think. intros; subst.
-          rewrite H; eauto. }
-          Qed.
-*)
-      Admitted.
      
-      Lemma typeof_env_length : forall g, 
-        length (typeof_env (types := types) g) = length g.
-      Proof.
-        clear. apply map_length.
-      Qed.
       Lemma implyEach_instantiate : forall HYPS U G,
         AllProvable funcs U G HYPS ->
         forall cc,
@@ -577,71 +705,193 @@ Module Make (SH : SepHeap) (U : SynUnifier).
         eapply IHHYPS; eauto.
       Qed. 
 
-(*  AllProvable funcs U G (map (U.exprInstantiate sub) (Hyps lem)). *)
-
-(*
-      Lemma checkAllInstantiated_lookup : forall sub ts from,
-        checkAllInstantiated from ts sub = true ->
-        forall tfuncs tU tG,
-          from = length tU ->
-          U.Subst_WellTyped tfuncs (tU ++ ts) tG sub ->
-          forall n t, 
-            nth_error ts n = Some t ->
-            exists e,
-            U.Subst_lookup (from + n) sub = Some e /\
-            is_well_typed tfuncs tU tG e t = true.
+      Lemma openForUnification_liftInstantiate : forall quant sub U e,
+        U.exprInstantiate sub (openForUnification U e) = liftInstantiate quant U 0 sub e.
       Proof.
-        induction ts using rev_ind; intros.
-          destruct n; simpl in *; unfold error in *; congruence.
+        induction e; simpl; intros; think;
+          repeat (rewrite U.exprInstantiate_Const || 
+                  rewrite U.exprInstantiate_Equal || 
+                  rewrite U.exprInstantiate_Func || 
+                  rewrite U.exprInstantiate_Not ||
+                  rewrite U.exprInstantiate_Var ||
+                  rewrite U.exprInstantiate_UVar);
+          think; auto.
+        { rewrite <- minus_n_O. reflexivity. }
+        { clear - H. f_equal. induction H; simpl; intros; think; auto. }
+      Qed.
 
-          
-(*
-        induction ts; simpl; intros. 
+      Lemma typeof_funcs_WellTyped_funcs_eq : forall tfuncs funcs,
+        WellTyped_funcs (types := types) tfuncs funcs ->
+        tfuncs = typeof_funcs funcs.
+      Proof.
+        clear. induction 1; auto. simpl. f_equal; auto. unfold WellTyped_sig, typeof_sig in *.
+        destruct r; destruct l; intuition; f_equal; auto.
+      Qed.
 
+      Lemma checkAllInstantiated_app : forall sub ts ts' from,
+        checkAllInstantiated from (ts ++ ts') sub = 
+        checkAllInstantiated from ts sub && checkAllInstantiated (length ts + from) ts' sub.
+      Proof.
+        clear. induction ts; simpl; intros; think; eauto; simpl.
+        consider (U.Subst_lookup from sub); intros; auto.
+        f_equal. rewrite Plus.plus_comm. simpl. rewrite Plus.plus_comm. reflexivity.
+      Qed.
+
+      Lemma Subst_to_env_app : forall U G sub ts ts' from, 
+        Subst_to_env U G sub (ts ++ ts') from = 
+        match Subst_to_env U G sub ts from , Subst_to_env U G sub ts' (length ts + from) with
+          | Some l , Some r => Some (l ++ r)
+          | _ , _ => None
+        end.
+      Proof.
+        induction ts; intros; simpl; think; auto.
+        destruct (Subst_to_env U G sub ts' from); auto.
+        cutrewrite (S (length ts + from) = length ts + S from); [ | omega ].
+        repeat match goal with 
+                 | [ |- context [ match ?X with _ => _ end ] ] => 
+                   match X with 
+                     | match _ with _ => _ end => fail 1
+                     | _ => destruct X
+                   end
+               end; auto.
+      Qed.
+
+      Lemma range_dropU : forall U G (e : expr types) t U',
+        is_well_typed (typeof_funcs funcs) (U ++ U') G e t = true ->
+        (forall n, n >= length U -> n < length U + length U' -> mentionsU n e = false) ->
+        is_well_typed (typeof_funcs funcs) U G e t = true.
+      Proof.
+        clear. induction U' using rev_ind; intros.
+        rewrite app_nil_r in *; auto.
+        rewrite <- app_ass in H. eapply is_well_typed_not_mentionsU_last in H. eapply IHU'; eauto.
+        intros. eapply H0; auto. rewrite app_length. simpl. omega.
+        eapply H0; rewrite app_length; try omega. rewrite app_length. simpl. omega.
+      Qed.
+
+      Lemma checkAllInstantiated_dropU : forall tU tG tfuncs sub ts ts',
+        checkAllInstantiated (length tU) ts sub = true ->
+        U.Subst_WellTyped tfuncs (tU ++ ts ++ ts') tG sub ->
+        forall e t n,
+          n >= length tU ->
+          is_well_typed tfuncs (tU ++ ts) tG e t = true ->
+          U.Subst_lookup n sub = Some e ->
+          is_well_typed tfuncs tU tG e t = true.
+      Proof.
+        clear. induction ts using rev_ind; simpl; intros; think; eauto.
+        rewrite app_nil_r in *. auto.
+        rewrite checkAllInstantiated_app in H. simpl in *; think. 
+        eapply IHts; eauto. rewrite app_ass in H0. simpl in *; eauto.
+        eapply is_well_typed_not_mentionsU_last. rewrite app_ass. eassumption.
+        eapply U.exprInstantiate_Removes. rewrite app_length. rewrite Plus.plus_comm; eauto.
+        instantiate (1 := e). eapply U.exprInstantiate_instantiated. eauto.
+      Qed.
+
+      Lemma checkAllInstantiated_Subst_to_env_success : forall U G tU tG tfuncs, 
+        WellTyped_env tU U ->
+        WellTyped_env tG G ->
+        WellTyped_funcs tfuncs funcs ->
+        forall sub ts ts',
+          checkAllInstantiated (length tU) (ts ++ ts') sub = true ->
+          U.Subst_WellTyped tfuncs (tU ++ ts ++ ts') tG sub ->
+          exists env, Subst_to_env U G sub ts (length tU) = Some env.
+      Proof.
+        clear; induction ts using rev_ind; simpl; intros; think; eauto.
+        { rewrite app_ass in *. simpl in *. generalize H2. eapply IHts in H2. 2: eauto.
+          destruct H2. rewrite Subst_to_env_app. rewrite H2. simpl.
+          intro XX. generalize XX. rewrite checkAllInstantiated_app in XX. simpl in XX. think.
+          generalize H5. eapply U.WellTyped_lookup in H5; eauto. destruct H5. intuition.
+          eapply checkAllInstantiated_dropU in XX. 5: eapply H7. 4: eauto.
+          3: omega. Focus 2. instantiate (1 := nil). repeat rewrite app_ass. simpl. rewrite app_nil_r. auto.
+          repeat rewrite nth_error_app_R in H8 by omega. repeat rewrite map_length in H8.
+          cutrewrite (length ts + length U - length U - length ts = 0) in H8; [ | omega ]. inversion H8. subst.
+          eapply is_well_typed_correct in XX.
+          4: eauto. 2: unfold WellTyped_env in *; auto. 2: unfold WellTyped_env in *; auto.
+          destruct XX. rewrite H5. eauto. }
+      Qed.
+      
+
+      (** TODO: lift this outside **)
+      Lemma fold_left_2_opt_unify : forall tU tG ts args args' sub sub',
+        U.Subst_WellTyped (types := types) (typeof_funcs funcs) tU tG sub -> 
+        all2 (is_well_typed (typeof_funcs funcs) tU tG) args ts = true ->
+        all2 (is_well_typed (typeof_funcs funcs) tU tG) args' ts = true ->
+        fold_left_2_opt (U.exprUnify unify_bound) args args' sub = Some sub' ->
+        U.Subst_WellTyped (typeof_funcs funcs) tU tG sub' /\
+        U.Subst_Extends sub' sub /\
+        map (U.exprInstantiate sub') args = map (U.exprInstantiate sub') args'.
+      Proof.
+        clear. induction ts; destruct args; destruct args'; intros; simpl in *; think; 
+        try (congruence || solve [ intuition (eauto; reflexivity) ]). 
+        do 2 generalize H2. apply U.exprUnify_sound in H2. intro. eapply U.exprUnify_Extends in H6.
+        intro. eapply U.exprUnify_WellTyped in H7; eauto. eapply IHts in H3; eauto. destruct H3.
+        intuition. etransitivity; eauto. rewrite H10. f_equal.
+        assert (U.exprInstantiate sub' (U.exprInstantiate s e) = U.exprInstantiate sub' (U.exprInstantiate s e0)).
+        rewrite H2. reflexivity. repeat rewrite U.exprInstantiate_Extends in H8 by eauto. auto.
+      Qed.
+
+      Lemma implyEach_sem : forall cc U G es,
+        implyEach es U G cc <-> (AllProvable funcs U G es -> cc).
+      Proof. clear; induction es; simpl; intuition. Qed.
+
+      Lemma liftInstantiate_lemmaD : forall quant BuildUVars BuildVars U G,
+        QuantifierSpec U G quant BuildUVars BuildVars ->
+        forall lem sub env,
+        Subst_to_env U G sub (Foralls lem) (length U) = Some env ->
+        lemmaD nil nil lem ->            
+        implyEach (map (liftInstantiate quant (length U) 0 sub) (Hyps lem)) U G
+        (forall specs : PropX.codeSpec (tvarD types pcType) (tvarD types stateType),
+          himp funcs preds nil env specs (Lhs lem) (Rhs lem)). 
+      Proof.
+        clear. destruct 3; simpl in *. eapply forallEachR_sem in H2; eauto using Subst_to_env_env.
+        eapply implyEach_sem. intros. eapply implyEach_sem in H2; eauto.
         
-          consider (U.Subst_lookup from sub); intros. specialize (IHts _ H3 tfuncs (tU ++ a :: nil) tG).
-          rewrite app_length in IHts. simpl length in IHts. rewrite plus_comm in IHts.
-          rewrite app_ass in IHts. simpl app in IHts. subst; specialize (IHts refl_equal H1).
-          destruct n; simpl in *. inversion H2; clear H2; subst. rewrite plus_0_r. eexists; split; eauto.
-          { admit. }
-          { eapply IHts in H2. destruct H2. intuition. clear IHts. rewrite plus_comm. simpl. rewrite plus_comm.
-            eexists; split; eauto.
- 
-          destruct n; simpl in *. inversion H4; clear H4; subst. rewrite plus_0_r in H3.
-
-
-inversion H3; clear H3; subst.
-          s
-*)
-      Admitted.
-*)
-
-      (* Lemma checkAllInstantiated_Subst_to_env_success : forall sub ts from, *)
-      (*   checkAllInstantiated from ts sub = true -> *)
-      (*   forall U G tfuncs tU tG, *)
-      (*     WellTyped_env tU U -> *)
-      (*     WellTyped_env tG G -> *)
-      (*     WellTyped_funcs tfuncs funcs -> *)
-      (*     U.Subst_WellTyped tfuncs (tU ++ ts) tG sub -> *)
-      (*     exists env, Subst_to_env U G sub ts from = Some env. *)
-      (* Proof. *)
-      (* Admitted. *)
-
-
-      Theorem applicableOk : forall asrt facts U G lem args args' sub TS,
-        all2 (is_well_typed (typeof_funcs funcs) (typeof_env U) (typeof_env G)) args TS = true ->
-        all2 (is_well_typed (typeof_funcs funcs) nil (Foralls lem)) args' TS = true ->
-        allb (fun e => is_well_typed (typeof_funcs funcs) nil (Foralls lem) e tvProp) (Hyps lem) = true ->
-        applicable unify_bound prover facts asrt (length U) lem args args' = Some sub ->
-        args = map (substExpr (length G) 0 sub) args' /\
-        AllProvable funcs U G (map (substExpr (length G) 0 sub) (Hyps lem)).
+        clear H2 specs. unfold WellTyped_lemma in *. think. generalize dependent (Hyps lem).
+        induction l; simpl; intros; auto. think. intuition. clear H6 H8.
+        unfold Provable in *.
+        generalize (liftInstantiate_spec H nil (F := env)). simpl. erewrite <- Subst_to_env_typeof_env by eassumption.
+        intro. eapply H6 in H1; eauto. rewrite H1.
+        consider (exprD funcs U G (liftInstantiate quant (length U) 0 sub a) tvProp); try contradiction; intros.
+        generalize (Weakenable _ nil _ _ H3). intro. rewrite H8. auto.
+      Qed.
+      Lemma allb_AllProvable : forall U G facts hyps,
+        Valid PC U G facts ->
+        allb (fun x => is_well_typed (typeof_funcs funcs) (typeof_env U) (typeof_env G) x tvProp) hyps = true ->
+        allb (Prove prover facts) hyps = true ->
+        AllProvable funcs U G hyps.
       Proof.
-(*
+        clear. induction hyps; simpl; intros; think; auto.
+        intuition; eauto. eapply Prove_correct; eauto. unfold ValidProp.
+        eapply is_well_typed_correct; eauto using typeof_env_WellTyped_env, typeof_funcs_WellTyped_funcs.
+      Qed.          
+      Lemma himp_existsEach_ST_EXT_existsEach : forall cs U P vars G,
+        ST.heq cs (sexprD funcs preds U G (SE.existsEach vars P)) 
+        (ST_EXT.existsEach vars (fun env => sexprD funcs preds U (rev env ++ G) P)).
+      Proof.
+        Opaque ST_EXT.existsEach.
+        induction vars; simpl; intros. rewrite ST_EXT.existsEach_nil. simpl. reflexivity.
+        change (a :: vars) with ((a :: nil) ++ vars). rewrite ST_EXT.existsEach_app.
+        rewrite ST_EXT.existsEach_cons. apply ST.heq_ex. intros. rewrite ST_EXT.existsEach_nil. rewrite IHvars.
+        simpl. eapply ST_EXT.heq_existsEach. intros. rewrite app_ass. reflexivity.
+      Qed.
 
- /\
+      Theorem applicableOk : forall quant (BuildUVars BuildVars : env types -> env types -> env types) U G,
+        QuantifierSpec U G quant BuildUVars BuildVars ->
+        forall cs facts lem args args' sub TS,
+        lemmaD nil nil lem ->
+        Valid PC U G facts ->
+        all2 (is_well_typed (typeof_funcs funcs) (typeof_env (types := types) U) (typeof_env G)) args TS = true ->
+        all2 (is_well_typed (typeof_funcs funcs) nil (Foralls lem)) args' TS = true ->
+(*        allb (fun e => is_well_typed (typeof_funcs funcs) nil (Foralls lem) e tvProp) (Hyps lem) = true -> *)
+        applicable unify_bound prover facts quant (length U) lem args args' = Some sub ->
+        args = map (liftInstantiate quant (length U) 0 sub) args' /\
         let (lq,lh) := hash (Lhs lem) in
         let (rq,rh) := hash (Rhs lem) in
-        himp funcs preds U G cs (existsEach lq (sheapD lh)) (existsEach rq (sheapD rh)).          
+        ST.himp cs (ST_EXT.existsEach lq (fun lq => 
+                       sexprD funcs preds (BuildUVars U (rev lq)) (BuildVars G (rev lq)) (*(G ++ lq)*)
+                       (sheapD (applySHeap (liftInstantiate quant (length U) (length lq) sub) lh))))
+                   (ST_EXT.existsEach rq (fun rq => 
+                       sexprD funcs preds (BuildUVars U (rev rq)) (BuildVars G (rev rq)) (*(G ++ lq)*)
+                       (sheapD (applySHeap (liftInstantiate quant (length U) (length rq) sub) rh)))).
       Proof.
         unfold applicable; intros.
         repeat match goal with
@@ -649,176 +899,122 @@ inversion H3; clear H3; subst.
                    consider X; try congruence; intros
                  | [ H : Some _ = Some _ |- _ ] => inversion H; clear H; subst
                end.
-        eapply all2_is_well_typed_weaken with (u := Foralls lem) (g := nil) in H0. apply andb_true_iff in H4. destruct H4.
-
-        cut (U.Subst_WellTyped (typeof_funcs funcs) (typeof_env U ++ Foralls lem) (typeof_env G) sub); intros.
-        { eapply checkAllInstantiated_Subst_to_env_success in H5.
-          5: eassumption.
-          2: eauto using typeof_env_WellTyped_env, typeof_funcs_WellTyped_funcs. 
-          2: eauto using typeof_env_WellTyped_env, typeof_funcs_WellTyped_funcs. 
-          2: eauto using typeof_env_WellTyped_env, typeof_funcs_WellTyped_funcs. 
-
-          destruct H5. destruct H.
-
-          Lemma Subst_to_env_typeof_env : forall U G sub TS cur x,
-            Subst_to_env U G sub TS cur = Some x ->
-            typeof_env x = TS.
+        eapply fold_left_2_opt_unify in H4. 2: apply U.Subst_empty_WellTyped.
+        Focus 2. eapply all2_impl. eassumption. intros. eapply is_well_typed_weaken with (u := Foralls lem) (g := nil).
+        eassumption.
+        Focus 2. rewrite all2_map_1. eapply all2_impl. eassumption. intros. 
+        rewrite <- typeof_env_length. eapply openForUnification_typed. eauto.
+        intuition.
+        {
+          Check Subst_to_env.
+          Lemma exprInstantiate_noop : forall sub (e : expr types),
+            (forall u, mentionsU u e = true -> U.Subst_lookup u sub = None) ->
+            U.exprInstantiate sub e = e.
           Proof.
-            induction TS; simpl; intros; 
-              repeat match goal with
-                       | [ H : Some _ = Some _ |- _ ] => inversion H; clear H; subst
-                       | [ H : context [ match ?X with _ => _ end ] |- _ ] =>
-                         consider X; intros
-                       | [ |- _ ] => progress ( simpl in * )
-                       | [ |- _ ] => f_equal ; [] 
-                     end; eauto; try congruence.
+            clear; induction e; simpl in *; intros; 
+              repeat (rewrite U.exprInstantiate_Const || 
+                  rewrite U.exprInstantiate_Equal || 
+                  rewrite U.exprInstantiate_Func || 
+                  rewrite U.exprInstantiate_Not ||
+                  rewrite U.exprInstantiate_Var ||
+                  rewrite U.exprInstantiate_UVar); think; try congruence; auto.
+            { rewrite H; auto. consider (beq_nat x x); auto. }
+            { f_equal. revert H0. induction H; simpl; intros; think; auto.
+              erewrite IHForall; try erewrite H; eauto; intros; eapply H1; think; auto using orb_true_r. }
+            { erewrite IHe1; try erewrite IHe2; eauto; intros; eapply H; think; auto using orb_true_r. }
           Qed.
-
-          Theorem unify_args_instantiate_equals : forall tfuncs tU tG l r D (S : U.Subst types) S',
-            fold_left_2_opt (U.exprUnify unify_bound) l r S = Some S' ->
-            U.Subst_WellTyped tfuncs tU tG S ->
-            all2 (@is_well_typed _ tfuncs tU tG) l D = true ->
-            all2 (@is_well_typed _ tfuncs tU tG) r D = true ->
-            map (U.exprInstantiate S') l = map (U.exprInstantiate S') r.
+          erewrite map_ext. 
+          2: intro; rewrite <- openForUnification_liftInstantiate; reflexivity.
+          Lemma independent_well_typed : forall sub F cU,
+            beq_nat (U.Subst_size sub) (length F) = true ->
+            checkAllInstantiated cU F sub = true ->
+            forall u, u <= cU -> U.Subst_lookup u sub = None.
           Proof.
-            induction l; destruct r; simpl; intros; think; auto. intros; subst; think. intros.
-            f_equal. admit.
-            eapply IHl; eauto. eapply U.exprUnify_WellTyped; eauto.
+          Admitted.
+          think. generalize (independent_well_typed _ _ H5 H8). 
+          revert H9. revert H2. clear. revert args'; revert TS.
+          induction args; destruct args'; destruct TS; simpl in *; intros; think; try congruence.
+          inversion H9. erewrite <- IHargs; eauto. f_equal. symmetry. eapply exprInstantiate_noop; eauto.
+          intros. eapply H.
+          Lemma is_well_typed_mentionsU : forall U G (e : expr types) t,
+            is_well_typed (typeof_funcs funcs) U G e t = true ->
+            forall u, mentionsU u e = true -> u < length U.
+          Proof.
+            clear. induction e; simpl; intros; try solve [ think; auto ].
+            think. apply nth_error_Some_length in H. auto.
+            admit.
+            { destruct t0. apply andb_true_iff in H. apply orb_true_iff in H0. destruct H. destruct H0; eauto. congruence. }
+            { destruct t; try congruence. eapply IHe; eauto. }
           Qed.
-          match goal with
-            | [ |- ?P /\ _ ] => assert (P); [ | split; [ assumption | ] ]
-          end.
-          
-          Check exprSubstU.
-          eapply unify_args_instantiate_equal
+          eapply is_well_typed_mentionsU in H2. 2: eauto. rewrite typeof_env_length in H2. omega. }
+        { consider (hash (Lhs lem)); consider (hash (Rhs lem)); intros; think.
+          generalize (@checkAllInstantiated_Subst_to_env_success _ _ _ _ _
+            (typeof_env_WellTyped_env U) (typeof_env_WellTyped_env G) (typeof_funcs_WellTyped_funcs funcs) sub (Foralls lem) nil).
+          rewrite app_nil_r in *. intro. destruct H12. rewrite typeof_env_length; auto. auto.
 
-          Lemma substExpr_exprInstantiate_exprSubstU : forall tF tU tG sub e t,
-            is_well_typed tF tU tG e t = true ->
-            substExpr (length tU) 0 sub e = U.exprInstantiate sub (exprSubstU 0 (length tG) (length tU) e).
-          Proof.
-            induction e; simpl; intros; think; intros; think.
-            { admit. }
-            { consider (NPeano.ltb x Y); intros.
-          
-
-          Theorem unify_args_forallEachR : forall tfuncs tU tG U G l r D (S : U.Subst types) S' P env cur TS,
-            U.Subst_WellTyped tfuncs tU tG S ->
-            all2 (@is_well_typed _ tfuncs tU tG) l D = true ->
-            all2 (@is_well_typed _ tfuncs tU tG) r D = true ->
-            fold_left_2_opt (fun l r => U.exprUnify unify_bound l (exprSubstU 0 (length TS) (length U) r)) l r S = Some S' ->
-            Subst_to_env U G S' TS cur = Some env ->
-            forallEachR TS P ->
-            map (U.exprInstantiate S') l = map (substExpr (length G) 0 S') r /\
-            P env.
-          Proof.
-            clear.
-            induction l; destruct r; try congruence; simpl in *; intros; think; intros; try solve [ intuition ].
-            { intuition. destruct TS; simpl in *. inversion H3; subst; intuition. think; intros. think; intros; think; intros.
-              think. eapply forallEachR_sem in H4. eauto. eapply Subst_to_env_typeof_env; eauto. }
-            { think. intros; subst; simpl in *.
-              eapply IHl in H6. 6: eauto. 3: eauto. 3: eauto. 3: eauto. intuition. rewrite H0. f_equal; auto.
-
-
-
-            { think; intuition. }
-            { think; intuition. think. consider (exprD funcs U G e t); intros; try congruence. inversion H6; subst.
-              eapply forallEachR_sem in H4. eapply H4. 
-
-              eapply Subst_to_env_typeof_env; eauto. }
-            { think; intuition; think; intuition. subst. simpl in *. think. intros. eapply IHl in H7; eauto.
-              
-
-(*
-              repeat match goal with
-                       | [ H : Some _ = Some _ |- _ ] => inversion H; clear H; subst
-                       | [ H : context [ match ?X with _ => _ end ] |- _ ] =>
-                         revert H ; case_eq X ; intros; try congruence
-                       | [ |- _ ] => progress ( simpl in * )
-                       | [ |- _ ] => progress subst
-                       | [ H : U.exprUnify _ _ _ _ = Some _ |- _ ] => 
-                         generalize H ; generalize H; 
-                           apply U.exprUnify_Extends in H ;
-                             let H := fresh "H" in
-                               intro H ;
-                                 apply U.exprUnify_sound in H
-                     end; try solve [ intuition ]. *) 
-            { intuition. eapply forallEachR_sem; eauto. simpl. admit. }
-            { intros.
-
-
-            eapply forallEachR_sem in H4. eapply H4.
-            eauto using Subst_to_env_env.        
+          rewrite typeof_env_length in H12. generalize H0. eapply liftInstantiate_lemmaD with (quant := quant) in H0; eauto.
+          intro.
+          eapply implyEach_sem in H0.
+          { specialize (H0 cs). 
+            rewrite SH.hash_denote in H0. rewrite H10 in H0.
+            rewrite SH.hash_denote with (s := Rhs lem) in H0. rewrite H8 in H0. simpl in H0.
             
-            intro. eapply IHl in H4. eapply H4. 4: eauto. eauto using U.exprUnify_WellTyped. eauto. eauto. eauto.
-          Qed.
-
-
-
-
-
-          eapply unify_args_forallEachR in H2; eauto using U.Subst_empty_WellTyped.
-          { simpl in *. 
-
-
-          }
-          
-
-
-          Focus 2.
-          { rewrite all2_map_1. eapply all2_impl. eauto.
-            clear H7 H H0 H2. induction x0; simpl; intros; think; auto. intros.
-            { consider (equiv_dec y t); think. unfold equiv in *. subst.
-              consider (NPeano.ltb x0 (length (Foralls lem))); intros; simpl. rewrite <- typeof_env_length.
-              rewrite nth_error_app_R by omega.
-              cutrewrite (length (typeof_env U) + x0 - 0 - length (typeof_env U) = x0). 2: omega. rewrite H.
-              destruct (equiv_dec t t); congruence.
-              exfalso. apply nth_error_Some_length in H. omega. }
-            { intros; think. exfalso. apply nth_error_Some_length in H. simpl in *. omega. }
-            { (* intros; think. unfold equiv in *; subst. induction H; simpl; think; auto.
-                 destruct (TDomain t); intros; try congruence.
-                 consider (is_well_typed (typeof_funcs funcs) nil (Foralls lem) x0 t0); intros.  *) admit. }
-            { intros; think. auto. } }
-          simpl in *.
-            
-
-
-clear. intros. rewrite <- app_nil_l with (l := Foralls lem) in H.
-          eapply is_well_typed_weaken with (u := typeof_env U) (g := nil) in H. rewrite app_nil_r in H.
-          eapply exprSubstU_WellTyped in H. simpl in *. eapply is_well_typed_weaken with (g := typeof_env G) (u := nil) in H.
-          repeat rewrite app_nil_r in *. simpl in *.
-
-          rewrite typeof_env_length in H. eassumption.
-          simpl in *.
-eapply H2. unfold hypD. unfold Provable in H.
-
-consider (exprD funcs nil x a tvProp); intros.
-            admit. 
-            Lemma Subst_to_env_typeof_env : forall U G sub TS cur x,
-              Subst_to_env U G sub TS cur = Some x ->
-              typeof_env x = TS.
+            destruct H13. clear H14. unfold WellTyped_lemma in *. think.
+            unfold himp in H0.
+            rewrite himp_existsEach_ST_EXT_existsEach in H0.
+            rewrite himp_existsEach_ST_EXT_existsEach in H0.
+            etransitivity. etransitivity; [ | eapply H0 ].
+            eapply ST.heq_defn. eapply ST_EXT.heq_existsEach; intros.
+            SearchAbout liftInstantiate.
+            Lemma applySHeap_spec : forall cs U G U' G' s F,
+              (forall e t, 
+                is_well_typed (typeof_funcs funcs) (typeof_env U) (typeof_env G) e t = true ->
+                exprD funcs U G e t = exprD funcs U' G' (F e) t) ->
+              SE.ST.heq cs (sexprD funcs preds U G (sheapD s))
+                           (sexprD funcs preds U' G' (sheapD (applySHeap F s))).
             Proof.
-              induction TS; simpl; intros; 
-                repeat match goal with
-                         | [ H : Some _ = Some _ |- _ ] => inversion H; clear H; subst
-                         | [ H : context [ match ?X with _ => _ end ] |- _ ] =>
-                           consider X; intros
-                         | [ |- _ ] => progress ( simpl in * )
-                         | [ |- _ ] => f_equal ; [] 
-                       end; eauto; try congruence.
-            Qed.
-            eapply Subst_to_env_typeof_env in H. subst.
-            eapply is_well_typed_correct in H1; eauto using typeof_env_WellTyped_env, typeof_funcs_WellTyped_funcs.
-            2: instantiate (1 := nil); reflexivity.
-            destruct H1; congruence.
-          Qed.
-
-          eapply implyEach_instantiate in H2. 
-          
-        
+(*
+              clear. intros. do 2 rewrite SH.sheapD_def. simpl. repeat eapply SE.ST.heq_star_frame.
+              { eapply MM.PROPS.map_induction with (m := impures s); intros.
+                repeat rewrite SH.impuresD_Empty by eauto using MF.map_Empty. reflexivity.
+                rewrite SH.impuresD_Add by eauto using MF.map_Add, MF.map_not_In.
+                symmetry. unfold MM.mmap_map in *. rewrite SH.impuresD_Add. 2: eapply MF.map_Add; eauto. 
+                2: eapply MF.map_not_In; eauto.
+                simpl. symmetry. apply ST.heq_star_frame; eauto.
+                cut (ST.heq cs (sexprD funcs preds U G SE.Emp) (sexprD funcs preds U' G' SE.Emp)); [ | reflexivity ].
+                generalize (@SE.Emp types pcType stateType). revert H. clear.
+                induction e; simpl; intros. repeat rewrite starred_nil. auto.
+                repeat rewrite starred_cons. simpl. apply ST.heq_star_frame; eauto. 
+                destruct (nth_error preds x); try reflexivity.
+                rewrite applyD_map. erewrite applyD_impl. reflexivity. intros. simpl. eauto. }
+              { cut (ST.heq cs (sexprD funcs preds U G SE.Emp) (sexprD funcs preds U' G' SE.Emp)); [ | reflexivity ].
+                generalize (@SE.Emp types pcType stateType). induction (pures s); intros; 
+                repeat (rewrite starred_nil || rewrite starred_cons); auto. simpl map. rewrite starred_cons.
+                simpl. rewrite IHl; eauto. rewrite H. reflexivity. }
+              { cut (ST.heq cs (sexprD funcs preds U G SE.Emp) (sexprD funcs preds U' G' SE.Emp)); [ | reflexivity ].
+                generalize (@SE.Emp types pcType stateType). induction (other s); intros.
+                etransitivity. rewrite starred_nil. reflexivity. etransitivity; [ | rewrite starred_nil; reflexivity ].
+                auto.
+                
+                etransitivity; [ rewrite starred_cons; reflexivity | ].
+                etransitivity; [ |  rewrite starred_cons; reflexivity ]. simpl. rewrite IHl; eauto. reflexivity. }
 *)
-      Admitted.
-
-
+            Admitted.
+            rewrite applySHeap_spec. reflexivity. intros. rewrite <- rev_length with (l := G0).
+            eapply liftInstantiate_spec; eauto.
+            Lemma typeof_env_app : forall l r,
+              typeof_env (types := types) l ++ typeof_env r = typeof_env (l ++ r).
+            Proof.
+              clear; induction l; simpl; intros; think; auto.
+            Qed.
+            rewrite typeof_env_app. assumption.
+            eapply ST.heq_defn. eapply ST_EXT.heq_existsEach; intros.
+            rewrite <- applySHeap_spec. reflexivity. intros. rewrite <- rev_length with (l := G0).
+            rewrite <- typeof_env_app in H17. eapply liftInstantiate_spec; eauto. }
+          { destruct H13. clear H14. unfold WellTyped_lemma in H13. eapply allb_AllProvable; eauto.
+            admit. (* think. revert H13. induction (Hyps lem); simpl; intros; auto; think
+            rewrite andb_true_r. generalize (liftInstantiate_typed U G). *) } }
+      Qed.
 
       Lemma app_len_2 : forall T (a b c d : list T),
         a ++ b = c ++ d ->
@@ -863,6 +1059,84 @@ consider (exprD funcs nil x a tvProp); intros.
                end; simpl. eexists; intuition.
       Qed.
 
+      Lemma skipn_length_gt : forall T (ls : list T) n,
+        length ls <= n ->
+        skipn n ls = nil.
+      Proof.
+        clear. induction ls; destruct n; simpl; intuition; auto.
+      Qed.
+
+      Lemma skipn_length_all : forall T U (F : T -> U) ls ls',
+        map F ls = ls' ->
+        skipn (length ls) ls' = nil.
+      Proof.
+        clear; intros. eapply skipn_length_gt. rewrite <- H. rewrite map_length. omega.
+      Qed.
+
+      Lemma rw_skipn_app : forall T (ls ls' : list T) n,
+        length ls = n ->
+        skipn n (ls ++ ls') = ls'.
+      Proof.
+        clear. induction ls; destruct n; simpl in *; intros; auto; congruence. 
+      Qed.
+      Lemma length_equal_map_rev : forall T U (F : T -> U) ls ls',
+        map F ls' = rev ls ->
+        length ls = length ls'.
+      Proof.
+        clear. intros. rewrite <- rev_length. rewrite <- H. rewrite map_length. auto.
+      Qed.
+      Hint Resolve length_equal_map_rev : list_length.
+      Lemma eq_proves_gt : forall a b,
+        a = b -> a <= b.
+      Proof.
+        clear. intros; omega.
+      Qed.
+      Lemma map_length_hint : forall T U (F : T -> U) a b,
+        map F a = b -> length b = length a.
+      Proof.
+        clear. intros. subst. rewrite map_length. auto.
+      Qed.
+      Hint Resolve eq_proves_gt map_length_hint skipn_length_gt : list_length.
+
+      Hint Resolve skipn_length_all : list_length.
+      Hint Rewrite skipn_length_all using (eauto with list_length) : list_length.
+
+      Lemma quantFwd_spec : forall U G (F : env types) (v : var) (t : tvar),
+        is_well_typed (typeof_funcs funcs) nil (typeof_env F) (Var (types := types) v) t = true ->
+        exprD funcs nil F (Var v) t =
+        exprD funcs U (G ++ F) (quantFwd (length (typeof_env G)) v) t.
+      Proof.
+        clear. simpl. unfold lookupAs; intros. think.
+        unfold typeof_env in H; rewrite map_nth_error_full in H.
+        rewrite typeof_env_length.
+        rewrite nth_error_app_R by omega. cutrewrite (v + length G - length G = v); [ | omega ].
+        destruct (nth_error F v); auto.
+      Qed.
+      Lemma hintSideD_In : forall hs,
+        hintSideD hs -> forall x, In x hs -> lemmaD nil nil x.
+      Proof.
+        clear. induction 1. inversion 1.
+        intros. inversion H1; subst; auto.
+      Qed.
+      Lemma applySHeap_singleton : forall meta_env vars_env cs F f l,
+        heq funcs preds meta_env vars_env cs
+        (sheapD (applySHeap F
+          {| impures := MM.mmap_add f l (MM.empty (list (expr types)))
+            ; pures := nil
+            ; other := nil |}))
+        (sheapD 
+          {| impures := MM.mmap_add f (map F l) (MM.empty (list (expr types)))
+            ; pures := nil
+            ; other := nil |}).
+      Proof.
+        clear. intros. unfold applySHeap; simpl. repeat rewrite SH.sheapD_def; simpl.
+        heq_canceler. unfold MM.mmap_add. repeat rewrite MM.FACTS.empty_o.
+        rewrite impuresD_Add with (f := f) (argss := map F l :: nil) (i := MM.empty _). symmetry. 
+        rewrite impuresD_Add with (f := f) (argss := map F l :: nil) (i := MM.empty _). reflexivity.
+        red; reflexivity. intro; eapply MM.FACTS.empty_in_iff; eassumption.
+        red; reflexivity. intro; eapply MM.FACTS.empty_in_iff; eassumption.
+      Qed.
+
       Opaque ST_EXT.existsEach.
 
       Lemma unfoldForwardOk : forall meta_env vars_env cs facts P Q,
@@ -870,11 +1144,10 @@ consider (exprD funcs nil x a tvProp); intros.
         WellTyped_env (Vars P) vars_env ->
         Valid PC meta_env vars_env facts ->
         unfoldForward unify_bound prover facts (Forward hs) P = Some Q ->
-        ST.himp cs
-        (sexprD funcs preds meta_env vars_env (sheapD (Heap P)))
-        (ST_EXT.existsEach (skipn (length vars_env) (Vars Q))
-          (fun vars_ext : list {t : tvar & tvarD types t} =>
-            sexprD funcs preds meta_env (vars_env ++ vars_ext) (sheapD (Heap Q)))).
+        ST.himp cs (sexprD funcs preds meta_env vars_env (sheapD (Heap P)))
+                   (ST_EXT.existsEach (skipn (length vars_env) (Vars Q))
+                     (fun vars_ext : list {t : tvar & tvarD types t} =>
+                       sexprD funcs preds meta_env (vars_env ++ vars_ext) (sheapD (Heap Q)))).
       Proof.
         unfold unfoldForward. intros.
         repeat match goal with
@@ -903,45 +1176,35 @@ consider (exprD funcs nil x a tvProp); intros.
           destruct (MF.FACTS.eq_dec f y); reflexivity. intro. apply MM.FACTS.remove_in_iff in H5. intuition congruence.
           red. intros. repeat (rewrite MM.FACTS.add_o || rewrite MM.FACTS.remove_o). consider (MF.FACTS.eq_dec f y); subst; auto. 
           intro. apply MM.FACTS.remove_in_iff in H5. intuition congruence. }
-        Lemma hintSideD_In : forall hs,
-          hintSideD hs -> forall x, In x hs -> lemmaD nil nil x.
-        Proof.
-          clear. induction 1. inversion 1.
-          intros. inversion H1; subst; auto.
-        Qed.
+        assert (exists p, nth_error preds f = Some p /\ all2 (is_well_typed (typeof_funcs funcs) UVars0 Vars0) x1 (SDomain p) = true).
+        { admit. }
+        destruct H5. destruct H5.
 
-(*
-          eapply hintSideD_In in H2; eauto using ForwardOk.
-          destruct H2.
-          unfold WellTyped_lemma in *. think. simpl in H9. consider (nth_error (Predicates_typeof preds) f); intros.
-          destruct (@applicableOk facts meta_env vars_env x x1 l s t); eauto.
-          admit. rewrite map_length in H6. auto.
-          Check Subst_to_env.
-          cut (exists e, Subst_to_env meta_env vars_env s (Foralls x) (length meta_env) = Some e).
-          intro. destruct H13. eapply forallEachR_sem with (e := x3) in H5. 2: admit.
-          apply implyEach_instantiate in H5.
-          eapply unify_args_forallEachR in H4. 6: eapply H0. simpl in *.
-          SearchAbout fold_left_2_opt.
-*)
-        
-      Admitted.
+        eapply hintSideD_In in H2; eauto using ForwardOk.
+        assert (length UVars0 = length meta_env).
+        { unfold WellTyped_env in *. subst. rewrite map_length. auto. }
+        rewrite H9 in *. 
+        eapply (applicableOk (QuantifierSpec_Fwd meta_env vars_env) cs facts (*meta_env vars_env*)) in H6.
+        Focus 2. eauto.
+        Focus 2. eauto.
+        Focus 2. unfold WellTyped_env in *. rewrite H in H8. rewrite H0 in H8. eapply H8.
+        Focus 2. destruct H2. unfold WellTyped_lemma in H2. think. simpl in H12. unfold typeof_preds in H12.
+          rewrite map_nth_error_full in H12. rewrite H5 in H12. eapply H12.
+        { destruct H6. rewrite H3 in *. rewrite SH.hash_Func in H10. rewrite H7 in H10.
+          rewrite ST_EXT.existsEach_nil in H10.
+          rewrite SH.hash_denote with (s := Func f x1). rewrite SH.hash_Func.
+          unfold fst, snd, SE.existsEach. rewrite app_nil_r in H10. 
+          subst.
+          rewrite applySHeap_singleton in H10. simpl in H10. simpl. rewrite H10. clear H10.
+          rewrite ST_EXT.heq_pushIn. rewrite rw_skipn_app; eauto with list_length.
 
-      Lemma skipn_length_gt : forall T (ls : list T) n,
-        length ls <= n ->
-        skipn n ls = nil.
-      Proof.
-        clear. induction ls; destruct n; simpl; intuition; auto.
+          rewrite ST_EXT.existsEach_rev. eapply ST.heq_defn. eapply ST_EXT.heq_existsEach; intros.
+          rewrite <- star_SHeap_denote. simpl. apply ST.heq_star_frame. 
+          { admit.  (** This requires weakening **) }
+          { rewrite rev_involutive. unfold WellTyped_env in *. subst. repeat rewrite map_length.
+            cutrewrite (length v = length (rev G)). reflexivity.
+            rewrite <- rev_length. rewrite <- H6. rewrite map_length. rewrite rev_length. reflexivity. } }
       Qed.
-
-      Lemma skipn_length_all : forall T U (F : T -> U) ls ls',
-        map F ls = ls' ->
-        skipn (length ls) ls' = nil.
-      Proof.
-        clear; intros. eapply skipn_length_gt. rewrite <- H. rewrite map_length. omega.
-      Qed.
-
-      Hint Resolve skipn_length_all : list_length.
-      Hint Rewrite skipn_length_all using (eauto with list_length) : list_length.
       
       Lemma forwardLength : forall bound facts P Q,
         forward bound facts P = Q ->
@@ -960,31 +1223,6 @@ consider (exprD funcs nil x a tvProp); intros.
                    end. repeat rewrite app_ass. eauto. }
           { subst. exists nil; repeat rewrite app_nil_r; eauto. }
       Qed.
-
-      Lemma rw_skipn_app : forall T (ls ls' : list T) n,
-        length ls = n ->
-        skipn n (ls ++ ls') = ls'.
-      Proof.
-        clear. induction ls; destruct n; simpl in *; intros; auto; congruence. 
-      Qed.
-      Lemma length_equal_map_rev : forall T U (F : T -> U) ls ls',
-        map F ls' = rev ls ->
-        length ls = length ls'.
-      Proof.
-        clear. intros. rewrite <- rev_length. rewrite <- H. rewrite map_length. auto.
-      Qed.
-      Hint Resolve length_equal_map_rev : list_length.
-      Lemma eq_proves_gt : forall a b,
-        a = b -> a <= b.
-      Proof.
-        clear. intros; omega.
-      Qed.
-      Lemma map_length_hint : forall T U (F : T -> U) a b,
-        map F a = b -> length b = length a.
-      Proof.
-        clear. intros. subst. rewrite map_length. auto.
-      Qed.
-      Hint Resolve eq_proves_gt map_length_hint skipn_length_gt : list_length.
 
       Theorem forwardOk : forall cs bound facts P Q,
         forward bound facts P = Q ->
@@ -1474,44 +1712,3 @@ End Packaged.
 
 End Make.
 
-
-(*
-      Theorem unify_args' : forall tfuncs tU tG U G l r D R f  S S',
-        U.Subst_WellTyped tfuncs tU tG S ->
-        all2 (@is_well_typed _ tfuncs tU tG) l D = true ->
-        all2 (@is_well_typed _ tfuncs tU tG) r D = true ->
-        fold_left_2_opt (U.exprUnify unify_bound) l r S = Some S' ->
-        U.Subst_equations funcs U G S ->
-        @applyD types (exprD funcs U G) D (map (U.exprInstantiate S') l) R f =
-        @applyD types (exprD funcs U G) D (map (U.exprInstantiate S') r) R f /\
-        U.Subst_equations funcs U G S' /\
-        U.Subst_Extends S' S /\
-        U.Subst_WellTyped tfuncs tU tG S'.
-      Proof.
-        induction l; destruct D; try congruence; simpl in *; intros;
-          repeat match goal with
-                   | [ H : Some _ = Some _ |- _ ] => inversion H; clear H; subst
-                   | [ H : context [ match ?X with _ => _ end ] |- _ ] =>
-                     revert H ; case_eq X ; intros; try congruence
-                   | [ |- _ ] => progress ( simpl in * )
-                   | [ |- _ ] => progress subst
-                   | [ H : U.exprUnify _ _ _ _ = Some _ |- _ ] => 
-                     generalize H ; generalize H; 
-                     apply U.exprUnify_Extends in H ;
-                     let H := fresh "H" in
-                     intro H ;
-                     apply U.exprUnify_sound in H
-                 end; try solve [ intuition ].
-        { 
-          
-
-          generalize H4; generalize H4; apply U.exprUnify_Extends in H4; auto.
-          intro. eapply U.exprUnify_WellTyped in H7; eauto.
-
- generalize H4. eapply U.exprUnify_sound in H4.
-          
-          
-
-
-
-*)
